\subsection{Rosenbrock Method}

\begin{frame}
  \begin{block}{Rosenbrock Method}
    \begin{equation*}
    \left\{
    \begin{aligned}
      x_{n+1} &:= x_n + \tau \sum_{j=1}^s b_j k_j
      \\
      k_i &:= f\left( x_n + \tau \sum_{j=1}^{i-1} \alpha_{ij} k_j \right) + \tau \Jac \sum_{j=1}^i \gamma_{ij} k_j
      \qquad
      \text{for } i = 1, \ldots, s
      ,
    \end{aligned}
    \right.
    \end{equation*}
    where $\Jac := f'(x_n)$ denotes the Jacobian.
  \end{block}
\end{frame}

\begin{frame}
  \begin{equation*}
    E\dot X E = C^\T C + A^\T X E + E^\T X A - E^\T X BB^\T X E
  \end{equation*}
  %\newcommand\U{\makebox[\widthof{$X_n$}]{U}}
  \begin{align*}
    \Ricc(X_n) &= C^\T C + A^\T X_n E + E^\T X_n A - E^\T X_n BB^\T X_n E \\
    \Jac(U) &= (A - BB^\T X_n)^\T U E + E^\T U (A - BB^\T X_n)
  \end{align*}
  The Jacobian is a Lyapunov operator!
\end{frame}

\begin{frame}
  \frametitle{1st Order Method \parencite{Mena2007,Lang2017}}
  Substitute $K_1 = \frac{1}{\tau}(X_{n+1} - X_n)$ into the stage equation.
  \begin{equation*}
    \tilde A_n^\T X_{n+1} E + E^\T X_{n+1} \tilde A_n
    = - GSG^\T
  \end{equation*}
  \begin{align*}
    G &= \begin{bmatrix}
      C^\T & L
    \end{bmatrix}
    \\
    S &= \begin{bmatrix}
      I & . \\
      . & DL^\T BB^\T LD + \tfrac{1}{\tau} D
    \end{bmatrix}
  \end{align*}
\end{frame}

\begin{frame}{2nd Order Method \parencite{Lang2015,Mena2007}}
  \begin{equation*}
  \end{equation*}
\end{frame}

\begin{frame}
\begin{columns}
\column{0.5\textwidth}
\begin{block}{Autonomous Initial Value Problem}
  \begin{equation*}
  \left\{
  \begin{aligned}
    \dot x &= f(x) \\
    x(t_0) &= x_0
  \end{aligned}
  \right.
  \end{equation*}
\end{block}

\column{0.5\textwidth}
  \begin{block}{1st Order Method}
    \begin{equation*}
    \left\{
    \begin{aligned}
      x_{n+1} &= x_n + \tau k_1 \\
      (I - \gamma\tau \Jac) k_1 &= f(x_n)
    \end{aligned}
    \right.
    \end{equation*}
  \end{block}
  \begin{block}{2nd Order Method \parencite{Verwer1999}}
    \vspace*{-\baselineskip}
    \begin{equation*}
    \left\{
    \begin{aligned}
      x_{n+1} &= x_n + \tfrac{3}{2} \tau k_1 + \tfrac{1}{2} \tau k_2 \\
      (I - \gamma\tau \Jac) k_1 &= f(x_n) \\
      (I - \gamma\tau \Jac) k_2 &= f(x_n + \tau k_1) - 2k_1
    \end{aligned}
    \right.
    \end{equation*}
  \end{block}
\end{columns}
\end{frame}
